lean4/ProofChecker/ProofChecker/Data/ClauseDb.lean
@@ -1,7 +1,8 @@
-import Std.Data.HashMap
-import Lean
-
-import ProofChecker.PropForm
+import ProofChecker.Model.PropForm
+import ProofChecker.Model.PropVars
+import ProofChecker.Model.Cnf
+import ProofChecker.Data.HashMap.Extra
+import ProofChecker.Data.ICnf
 
 /-! Clause database together with some (TBD provably correct) methods. For example, we can conclude
 that if a clause follows from the current database by unit propagation, then it is implied by the
@@ -12,28 +13,13 @@ checkers such as for LRAT. It uses in-place data structures, so should be used l
 
 (Persistent structures do not seem immediately helpful as linear formats do not backtrack.)
 
-In `ClauseDb α β`, `α` is the type of clause indices and `β` is the type of literals.
-Later on, we require `Neg β` for negating literals. -/
-structure ClauseDb (α β : Type) [BEq α] [Hashable α] where
-  clauses : Std.HashMap α (Array β × Bool) := {}
-  -- LATER: which clauses a given literal occurs in.
-  -- occurs : Std.HashMap β (Array α)
+In `ClauseDb α`, `α` is the type of clause indices. -/
+structure ClauseDb (α : Type) [BEq α] [Hashable α] where
+  /-- Each clause is stored together with a flag indicating whether it has been deleted.
+  Deleted clauses are logically not in the database. -/
+  clauses : HashMap α (IClause × Bool) := {}
 
-/-- A partial assignment to propositional literals. It assigns directly to literals, so it be
-inconsistent. -/
--- TODO: is a lit-indexed Array Bool better?
-def PartPropAssignment (β : Type) := List β
-
-/-- Interpret the negation of a partial assignment as a clause. For example, x₁ ∧ -x₂ ↦ -x₁ ∨ x₂. -/
-def PartPropAssignment.interpNeg [Neg β] (τ : PartPropAssignment β) : PropForm β :=
-  -- TODO: how does consistency come in here? The negation must be well-behaved wrt evaluation;
-  -- maybe; or maybe it will not end up mattering later if we relativize to neg
-  τ.foldl (init := .fls) fun acc l => acc.disj (.var (-l))
-
-def Clause.interp (C : Array β) : PropForm β :=
-  C.foldl (init := .fls) fun acc l => acc.disj (.var l)
-
-namespace Std.HashMap
+namespace HashMap
 
 variable [BEq α] [Hashable α]
 
@@ -42,17 +28,19 @@ def mapOne (m : HashMap α β) (idx : α) (f : β → β) : HashMap α β :=
   | some b => m.insert idx (f b)
   | none => m
 
-end Std.HashMap
+end HashMap
 
-inductive UnitPropResult (α β : Type) where
+inductive UnitPropResult (α : Type) where
   | contradiction
-  /-- Either the hint did not become unit or it points at a nonexistent clause. -/
-  | wrongHint (hint : α)
-  | extended (τ : PartPropAssignment β)
+  /-- The hint did not become unit. -/
+  | hintNotUnit (hint : α)
+  /-- The hint points at a nonexistent clause. -/
+  | hintNonexistent (hint : α)
+  | extended (τ : PartPropAssignment)
 
 namespace UnitPropResult
 
-def isContradiction (r : UnitPropResult α β) : Bool :=
+def isContradiction (r : UnitPropResult α) : Bool :=
   r matches contradiction
 
 end UnitPropResult
@@ -61,60 +49,67 @@ namespace ClauseDb
 
 variable {α : Type} [BEq α] [Hashable α]
 
-instance [ToString α] [ToString β] : ToString (ClauseDb α β) where
+instance [ToString α] : ToString (ClauseDb α) where
   toString db := toString db.clauses.toList
 
-def empty : ClauseDb α β := { clauses := .empty }
+def empty : ClauseDb α := { clauses := .empty }
 
--- Detail: `PropForm β` has literals as variables. This makes it possible
--- to write down inconsistent assignments x ↦ ⊤, -x ↦ ⊤. We'll just require
--- `LawfulNeg` or something like that.
-def interp (db : ClauseDb α β) : PropForm β :=
-  db.clauses.fold (init := .tr) fun acc _ (cl, deleted) =>
-    if deleted then acc else acc.conj (Clause.interp cl)
+def fold (db : ClauseDb α) (f : β → α → IClause → β) (init : β) : β :=
+  db.clauses.fold (init := init) fun acc idx (C, deleted) =>
+    if deleted then acc else f acc idx C
 
-def addClause (db : ClauseDb α β) (idx : α) (C : Array β) : ClauseDb α β :=
+def foldM [Monad m] (db : ClauseDb α) (f : β → α → IClause → m β) (init : β) : m β :=
+  db.clauses.foldM (init := init) fun acc idx (C, deleted) =>
+    if deleted then pure acc else f acc idx C
+
+def addClause (db : ClauseDb α) (idx : α) (C : IClause) : ClauseDb α :=
   { db with clauses := db.clauses.insert idx (C, false) }
 
-def delClause (db : ClauseDb α β) (idx : α) : ClauseDb α β :=
+def delClause (db : ClauseDb α) (idx : α) : ClauseDb α :=
   { db with clauses := db.clauses.mapOne idx fun (C, _) => (C, true) }
 
-def getClause (db : ClauseDb α β) (idx : α) : Option (Array β) :=
+def getClause (db : ClauseDb α) (idx : α) : Option IClause :=
   db.clauses.find? idx |>.bind (fun (C, deleted) => if deleted then none else C) 
 
-def contains (db : ClauseDb α β) (idx : α) : Bool :=
+def contains (db : ClauseDb α) (idx : α) : Bool :=
   db.getClause idx |>.isSome
-
-theorem interp_addClause (db : ClauseDb α β) (idx : α) (C : Array β)
-    (h : db.clauses.contains idx = false)
-    : (db.addClause idx C).interp = db.interp.conj (Clause.interp C) :=
-  sorry
 
 /-- Propagates units starting from the given assignment. The clauses in `hints` are expected to become
 unit in the order provided. Returns the extended assignment, or `none` if a contradiction was found. -/
-def unitPropWithHints [BEq β] [Neg β] (db : ClauseDb α β) (τ : PartPropAssignment β) (hints : Array α)
-    : UnitPropResult α β := Id.run do
+def unitPropWithHints (db : ClauseDb α) (τ : PartPropAssignment) (hints : Array α)
+    : UnitPropResult α := Id.run do
   let mut τ := τ
   for hint in hints do
     let some C := db.getClause hint
-      | return .wrongHint hint
-    match reduceClause C τ with
-    | some [u] => τ := u :: τ
-    | some [] => return .contradiction
-    | _ => return .wrongHint hint
+      | return .hintNonexistent hint
+    match C.reduce τ with
+    | some #[u] => τ := τ.insert u.var u.polarity
+    | some #[] => return .contradiction
+    | _ => return .hintNotUnit hint
   return .extended τ
-where
-  /-- Reduces a clause by a partial assignment. Returns `none` if it became satisfied,
-  otherwise `some C'` where `C'` is the reduced clause. -/
-  reduceClause (C : Array β) (τ : PartPropAssignment β) : Option (List β) :=
-    C.foldlM (init := []) fun acc l =>
-      -- NOTE: linear in assignment size
-      match τ.find? (fun l' => l' == l || l' == -l) with
-      | none => l :: acc
-      | some l' => if l' == l then none else acc
+  
+/-! Theorems about `ClauseDb` -/
+  
+def toPropTerm (db : ClauseDb α) : PropTerm Nat :=
+  db.fold (init := .tr) fun acc _ C => acc.conj C.toPropTerm
 
-theorem entails_of_unitProp [BEq β] [Neg β] (db : ClauseDb α β) (τ : PartPropAssignment β)
-    (hints : Array α) : db.unitPropWithHints τ hints |>.isContradiction → db.interp ⊨ τ.interpNeg :=
+theorem toPropTerm_getClause (db : ClauseDb α) (idx : α) :
+    db.getClause idx = some C → db.toPropTerm.entails C.toPropTerm :=
+  sorry
+
+theorem toPropTerm_addClause (db : ClauseDb α) (idx : α) (C : IClause)
+    -- only true when idx ∉ db
+    : (db.addClause idx C).toPropTerm = db.toPropTerm.conj C.toPropTerm :=
+  sorry
+
+-- Not sure if true
+theorem toPropTerm_delClause (db : ClauseDb α) (idx : α) :
+    db.getClause idx = some C →
+    (db.delClause idx).toPropTerm.conj C.toPropTerm = db.toPropTerm :=
+  sorry
+
+theorem entails_of_unitProp (db : ClauseDb α) (τ : PartPropAssignment) (hints : Array α) :
+    db.unitPropWithHints τ hints |>.isContradiction → db.toPropTerm.entails (.neg τ.toPropTerm) :=
   sorry
 
 end ClauseDb
