lean4/ProofChecker/ProofChecker/Checker/CheckerCore.lean
@@ -1,0 +1,282 @@
+import Std.Data.Array.Basic
+
+import ProofChecker.Data.ClauseDb
+import ProofChecker.Data.PropGraph
+import ProofChecker.Data.HashSet
+
+/-- A step in a CRAT proof. -/
+inductive CratStep
+  | /-- Add asymmetric tautology. -/
+    addAt (idx : Nat) (C : IClause) (upHints : Array Nat)
+  | /-- Delete asymmetric tautology. -/
+    delAt (idx : Nat) (upHints : Array Nat)
+  | /-- Declare product operation. -/
+    prod (idx : Nat) (x : Nat) (ls : Array ILit)
+  | /-- Declare sum operation. -/
+    sum (idx : Nat) (x : Nat) (l₁ l₂ : ILit) (upHints : Array Nat)
+  | /-- Declare POG root. -/
+    root (r : Nat)
+
+namespace CratStep
+
+instance : ToString CratStep where
+  toString := fun
+    | addAt idx C upHints => s!"{idx} a {C} 0 (hints : {upHints})"
+    | delAt idx upHints => s!"dc {idx} (hints: {upHints})"
+    | prod idx x ls => s!"{idx} p {x} {ls}"
+    | sum idx x l₁ l₂ upHints => s!"{idx} s {x} {l₁} {l₂} (hints: {upHints})"
+    | root x => s!"r {x}"
+  
+-- TODO : toDimacs
+
+end CratStep
+
+/-- The checker's runtime state. Contains exactly the data needed to fully check a proof. -/
+structure CheckerStateCore where
+  inputCnf : ICnf
+  /-- Number of variables in the original CNF. -/
+  numOrigVars : Nat
+  /-- The clause database. -/
+  clauseDb : ClauseDb Nat := {}
+  /-- The dependency set of every variable currently present in the ClauseDb. -/
+  depVars : HashMap Nat (HashSet Nat) := {}
+  -- TODO: replace with ItegCount?
+  -- TODO: should the initial state include all original variables as disconnected verts?
+  scheme : PropDag Nat := .empty
+  /-- Which clauses are counting scheme definition clauses. -/
+  schemeDefs : HashSet Nat := .empty Nat
+  root : Option Nat := none
+
+inductive CheckerError where
+  | graphUpdateError (err : Dag.DagException Nat)
+  | duplicateClauseIdx (idx : Nat)
+  | unknownClauseIdx (idx : Nat)
+  | hintNotUnit (idx : Nat)
+  | hintNonexistent (idx : Nat)
+  | upNoContradiction (τ : PartPropAssignment)
+  | duplicateExtVar (x : Nat)
+  | unknownVar (x : Nat)
+  | depsNotDisjoint (xs : List Nat)
+  | finalRootNotSet
+  | finalClauseInvalid (idx : Nat) (C : IClause)
+
+namespace CheckerError
+
+instance : ToString CheckerError where
+  toString := fun
+    | graphUpdateError e => s!"graph update error: {e}"
+    | duplicateClauseIdx idx => s!"duplicate clause index: {idx}"
+    | unknownClauseIdx idx => s!"unknown clause index: {idx}"
+    | hintNotUnit idx => s!"hinted clause at {idx} did not become unit"
+    | hintNonexistent idx => s!"hinted clause at {idx} does not exist"
+    | upNoContradiction τ => s!"unit propagation did not derive contradiction (final assignment {τ.toList})"
+    | duplicateExtVar x => s!"extension variable '{x}' was already introduced"
+    | unknownVar x => s!"unknown variable '{x}'"
+    | depsNotDisjoint xs => s!"variables {xs} have non-disjoint dependency sets"
+    | finalRootNotSet => s!"proof done but root variable was not set"
+    | finalClauseInvalid idx C => s!"proof done but clause '{C}' at {idx} is neither the root nor a PDAG definition"
+
+end CheckerError
+
+abbrev CheckerCoreM := ExceptT CheckerError <| StateM CheckerStateCore
+
+def initial (inputCnf : ICnf) : CheckerStateCore :=
+  { inputCnf
+    numOrigVars := inputCnf.vars.size
+    clauseDb :=
+      let (db, _) := inputCnf.foldl (init := (.empty, 1))
+        fun (db, idx) C => (db.addClause idx C, idx + 1)
+      db
+    depVars := inputCnf.vars.fold (init := .empty) fun s x => s.insert x (.empty Nat)
+    scheme := inputCnf.vars.fold (init := .empty) fun s x => s.addVar x |>.toOption.get!
+  }
+
+/-- Check if `C` is an asymmetric tautology wrt the clause database. -/
+def checkAtWithHints (C : IClause) (hints : Array Nat) : CheckerCoreM Unit := do
+  let st ← get
+  match st.clauseDb.unitPropWithHints C.toFalsifyingAssignment hints with
+  | .contradiction => return ()
+  | .extended τ => throw <| .upNoContradiction τ
+  | .hintNotUnit hint => throw <| .hintNotUnit hint
+  | .hintNonexistent hint => throw <| .hintNotUnit hint
+
+-- NOTE: I'll likely have to rewrite uses of monadic sequencing into functional code because
+-- sequencing is non-dependent.
+
+def addClause (idx : Nat) (C : IClause) : CheckerCoreM Unit := do
+  let st ← get
+  if st.clauseDb.contains idx then
+    throw <| .duplicateClauseIdx idx
+  set { st with clauseDb := st.clauseDb.addClause idx C }
+
+def saveSchemeDef (idx : Nat) : CheckerCoreM Unit := do
+  let st ← get
+  set { st with schemeDefs := st.schemeDefs.insert idx }
+
+def addAt (idx : Nat) (C : IClause) (hints : Array Nat) : CheckerCoreM Unit := do
+  checkAtWithHints C hints
+  addClause idx C
+
+def delAt (idx : Nat) (hints : Array Nat) : CheckerCoreM Unit := do
+  let st ← get
+  let some C := st.clauseDb.getClause idx
+    | throw <| .unknownClauseIdx idx
+  set { st with clauseDb := st.clauseDb.delClause idx }
+  -- The clause is AT by everything except itself.
+  checkAtWithHints C hints
+
+def addProd (idx : Nat) (x : Nat) (ls : Array ILit) : CheckerCoreM Unit := do
+  let st ← get
+
+  -- Check that added variable is fresh.
+  if st.depVars.contains x then
+    throw <| .duplicateExtVar x
+
+  -- Check that variables are known and compute their dependencies.
+  let Ds ← ls.mapM fun l =>
+    match st.depVars.find? l.var with
+    | some D => pure D
+    | none => throw <| .unknownVar l.var
+
+  -- Compute total dependency set and check pairwise disjointness.
+  let (union, disjoint) := HashSet.Union' Ds
+  if !disjoint then
+    throw <| .depsNotDisjoint (ls.toList.map ILit.var)
+
+  -- Defining clauses for the conjunction.
+  addClause idx (ls.map (-·) |>.push (.mkPos x))
+  saveSchemeDef idx
+  let _ ← ls.mapIdxM fun i l => do
+    addClause (idx+1+i) #[.mkNeg x, l]
+    saveSchemeDef (idx+1+i)
+
+  modify fun st => { st with
+    depVars := st.depVars.insert x union
+    scheme := st.scheme.addConj x (ls.toList.map fun l => (l.polarity, l.var)) |>.toOption.get!
+  }
+
+def addSum (idx : Nat) (x : Nat) (l₁ l₂ : ILit) (hints : Array Nat) : CheckerCoreM Unit := do
+  let st ← get
+
+  -- Check that added variable is fresh.
+  if st.depVars.contains x then
+    throw <| .duplicateExtVar x
+
+  -- Check that variables are known and compute their dependencies.
+  let some D₁ := st.depVars.find? l₁.var
+    | throw <| .unknownVar l₁.var
+  let some D₂ := st.depVars.find? l₂.var
+    | throw <| .unknownVar l₂.var
+
+  -- Check that variables are mutually exclusive.
+  checkAtWithHints #[l₁.neg, l₂.neg] hints
+
+  -- Defining clauses for the disjunction.
+  addClause idx     #[.mkNeg x, l₁, l₂]
+  saveSchemeDef idx
+  addClause (idx+1) #[.mkPos x, -l₁]
+  saveSchemeDef (idx+1)
+  addClause (idx+2) #[.mkPos x, -l₂]
+  saveSchemeDef (idx+2)
+
+  modify fun st => { st with
+    depVars := st.depVars.insert x (D₁.union D₂)
+    scheme := st.scheme.addDisj x ([(l₁.polarity, l₁.var), (l₂.polarity, l₂.var)]) |>.toOption.get!
+  }
+
+def setRoot (r : Nat) : CheckerCoreM Unit := do
+  modify fun st => { st with root := some r }
+
+def checkFinalState : CheckerCoreM Unit := do
+  let st ← get
+
+  let some r := st.root
+    | throw <| .finalRootNotSet
+
+  let _ ← st.clauseDb.foldM (init := ()) fun _ idx C => do
+    if C != #[.mkPos r] && !st.schemeDefs.contains idx then
+      throw <| .finalClauseInvalid idx C
+
+def checkProofStep (step : CratStep) : CheckerCoreM Unit :=
+  match step with
+  | .addAt idx C hints => addAt idx C hints
+  | .delAt idx hints => delAt idx hints
+  | .prod idx x ls => addProd idx x ls
+  | .sum idx x l₁ l₂ hints => addSum idx x l₁ l₂ hints
+  | .root r => setRoot r
+
+-- def count (r : Nat) : CheckerCoreM Nat := do
+--   let st ← get
+--   st.scheme.count r st.numOrigVars
+
+def checkProof (cnf : ICnf) (pf : Array CratStep) : Except CheckerError Unit := do
+  let mut st : CheckerStateCore := initial cnf
+  let x : CheckerCoreM Unit := do
+    for step in pf do
+      checkProofStep step
+    checkFinalState
+  let (ret, _) := x.run st |>.run
+  ret
+
+-- For relating the scheme defining clauses to the the actual scheme
+def schemeDefsToPropTerm : CheckerCoreM (PropTerm Nat) := do
+  let st ← get
+  return st.schemeDefs.fold (init := .tr) (fun acc idx =>
+    let C := st.clauseDb.getClause idx |>.getD #[]
+    acc.conj C.toPropTerm)
+
+/-- The given checker state is well-formed. -/
+structure CheckerStateWF (st : CheckerStateCore) : Prop where
+  -- fresh variables
+  -- ∀ x : Nat, x ∈ st.clauseDb.toPropTerm.depVars → st.depVars.contains x
+  -- corollary: if not in depVars then does not influence func and can be used as extension var
+
+  -- logical equivalence
+  -- let X0 := st.inputCnf.toPropForm.vars
+  -- equivalentOver X0 st.inputCnf.toPropForm st.clauseDb.toPropForm
+  -- hasUniqueExtension X0 st.clauseDb.toPropForm.vars st.clauseDb.toPropForm
+
+  -- compatibility between clauses and schema
+  -- ∀ x : Nat, equivalentOver X0 (.conj x st.schemaToPropForm) (st.scheme.toPropForm x)
+
+  -- decomposability
+  -- ∀ x : Nat, st.scheme.toPropForm x |>.decomposable
+
+#exit
+
+-- TODO: re-add tracing in a way compatible with WF-subtyping
+
+/-- Wraps a well-formed checker state with extra stuff for actually running and debugging it. -/
+structure CheckerState where
+  core : CheckerStateCore
+  wf : CheckerStateWF core
+  verbose : Bool := false
+  trace : Array String := #[]
+
+namespace CheckerState
+
+-- Problem: functions like addClause temporarily break invariants, so can't live in CheckerWFM
+-- Solution (?): write CheckerWFM and a lift from CheckerM that takes a proof of the invariants
+-- being preserved
+
+abbrev CheckerM := ExceptT CheckerError <| StateM CheckerState
+
+def withTraces (f : Array String → String) (x : CheckerM Unit) : CheckerM Unit := do
+  if (← get).verbose then
+    let prevTrace ← modifyGet fun st => (st.trace, { st with trace := #[] })
+    try x
+    finally
+      modify fun st => { st with trace := prevTrace.push <| f st.trace }
+  else
+    x
+
+def log_ (msg : Unit → String) : CheckerM Unit := do
+  modify fun st =>
+    if st.verbose then { st with trace := st.trace.push <| msg () }
+    else st
+
+syntax "log! " interpolatedStr(term) : term
+macro_rules
+  | `(log! $interpStr) => `(log_ fun _ => s!$interpStr)
+
+end CheckerState
