lean4/ProofChecker/ProofChecker/Checker/Parse.lean
@@ -1,0 +1,153 @@
+import ProofChecker.Data.ICnf
+import ProofChecker.Checker.CheckerCore
+
+def Except.ofOption (e : ε) : Option α → Except ε α
+  | none   => .error e
+  | some x => .ok x
+
+namespace Dimacs
+
+inductive Token where
+  | int (i : Int) | str (s : String)
+  deriving Repr, BEq
+
+instance : Coe String Token :=
+  ⟨Token.str⟩
+
+instance : Coe Int Token :=
+  ⟨Token.int⟩
+
+instance : ToString Token where
+  toString := fun | .int v | .str v => toString v
+
+def Token.getInt? : Token → Option Int
+  | .int i => some i
+  | .str _ => none
+
+def Token.getStr? : Token → Option String
+  | .int _ => none
+  | .str s => some s
+
+def tokenizeLines (lines : Array String) : Array (Array Token) := Id.run do
+  let mut lns := #[]
+  for ln in lines do
+    let tks := ln.splitOn " " |>.filter (· ≠ "")
+    if tks.isEmpty then continue
+    if tks.head! == "c" then continue
+    let mut ln := #[]
+    for tk in tks do
+      if let some i := tk.toInt? then
+        ln := ln.push <| .int i
+      else
+        ln := ln.push <| .str tk
+    lns := lns.push ln
+  return lns
+
+end Dimacs
+
+open Dimacs
+
+def ILit.ofToken : Token → Except String ILit
+  | .int i => .ok i
+  | .str s => .error s!"expected int at '{s}'"
+  
+def Nat.ofToken : Token → Except String Nat
+  | .int i =>
+    if i < 0 then .error s!"expected positive int at '{i}'"
+    else .ok (Int.natAbs i)
+  | .str s => .error s!"expected int at '{s}'"
+
+def IClause.ofTokens (tks : Array Token) : Except String IClause := do
+  tks.mapM ILit.ofToken
+
+/-- Return a CNF computed from the tokens of a DIMACS CNF file. -/
+def ICnf.ofLines (lns : Array (Array Token)) : Except String ICnf := do
+  let some hdr := lns[0]? 
+    | throw s!"expected at least one line"
+  -- TODO: Check nVars
+  let #[.str "p", .str "cnf", .int nVars, .int nClauses] := hdr
+    | throw s!"unexpected header {hdr}"
+  let mut clauses : ICnf := #[]
+  for ln in lns[1:] do
+    try
+      let some (.int 0) := ln[ln.size - 1]?
+        | throw s!"missing terminating 0"
+      let lits := ln[:ln.size - 1]
+      let clause ← IClause.ofTokens lits
+      clauses := clauses.push clause
+    catch e =>
+      throw s!"error on line '{ln}': {e}"
+  if Int.ofNat clauses.size ≠ nClauses then
+    throw s!"expected {nClauses} clauses, but got {clauses.size}"
+  return clauses
+
+def ICnf.readDimacsFile (fname : String) : IO ICnf := do
+  let lns ← IO.FS.lines fname
+  let lns := Dimacs.tokenizeLines lns
+  match ofLines lns with
+  | .ok v => return v
+  | .error e => throw <| IO.userError e
+  
+/-- Return a proof step given a DIMACS line. -/
+def CratStep.ofTokens (tks : Array Token) : Except String CratStep := do
+  let toUpHints (tks : Array Token) : Except String (Array Nat) := do
+    if let #[.str "*"] := tks then
+      throw s!"got unhinted proof, but all hints need to be filled in"
+    tks.mapM Nat.ofToken
+  let (some fst, some snd) := (tks[0]?, tks[1]?)
+    | throw s!"expected at least two tokens"
+  let tks := tks[2:]
+  match fst, snd with
+  | idx, .str "a" =>
+    let C := Array.takeWhile (· != Token.int 0) tks
+    let some (.int 0) := tks[C.size]?
+      | throw s!"missing terminating 0 in clause"
+    let some (.int 0) := tks[tks.size-1]?
+      | throw s!"missing terminating 0 in hints"
+    let hints : Subarray Token := tks[C.size+1:tks.size-1]
+    return .addAt (← Nat.ofToken idx) (← IClause.ofTokens C) (← toUpHints hints)
+  | .str "dc", idx =>
+    let some (.int 0) := tks[tks.size-1]?
+      | throw s!"missing terminating 0 in hints"
+    let hints : Subarray Token := tks[:tks.size-1]
+    return .delAt (← Nat.ofToken idx) (← toUpHints hints)
+  | idx, .str "p" =>
+    let some x := tks[0]?
+      | throw s!"missing product literal"
+    let some (.int 0) := tks[tks.size-1]?
+      | throw s!"missing terminating 0 in hints"
+    let ls : Subarray Token := tks[1:tks.size-1]
+    return .prod (← Nat.ofToken idx) (← Nat.ofToken x) (← IClause.ofTokens ls)
+  | idx, .str "s" =>
+    let (some x, some l₁, some l₂) := (tks[0]?, tks[1]?, tks[2]?)
+      | throw s!"missing sum parameters"
+    let some (.int 0) := tks[tks.size-1]?
+      | throw s!"missing terminating 0 in hints"
+    let hints : Subarray Token := tks[3:tks.size-1]
+    return .sum (← Nat.ofToken idx) (← Nat.ofToken x) (← ILit.ofToken l₁) (← ILit.ofToken l₂)
+      (← toUpHints hints)
+  | .str "r", r =>
+    return .root (← Nat.ofToken r)
+  | .str "do", _ => throw s!"do command is not supported"
+  | _, .str "i" => throw s!"i command is deprecated"
+  | _, _ => throw s!"unexpected command"
+
+def CratStep.readDimacsFile (fname : String) : IO (Array CratStep) := do
+  let lns ← IO.FS.lines fname
+  let lns := Dimacs.tokenizeLines lns
+  let mut pf := #[]
+  for ln in lns do
+    match CratStep.ofTokens ln with
+    | .ok v => pf := pf.push v
+    | .error e => throw <| IO.userError s!"error on line '{ln}': {e}"
+  return pf
+  
+def CratStep.toDimacs : CratStep → String
+  | addAt idx C upHints => s!"{idx} a {pArray C} 0 {pArray upHints} 0"
+  | delAt idx upHints => s!"dc {idx} {pArray upHints} 0"
+  | prod idx x ls => s!"{idx} p {x} {pArray ls} 0"
+  | sum idx x l₁ l₂ upHints => s!"{idx} s {x} {l₁} {l₂} {pArray upHints} 0"
+  | root x => s!"r {x}"
+where
+  pArray {α : Type} [ToString α] (a : Array α) :=
+    " ".intercalate (a.foldr (init := []) fun a acc => toString a :: acc)
